Refactor constr prop

theories/ValueOpts/ConstantPropagationAnalysis.v
@@ -4,7 +4,7 @@ Require Import Plus Util AllInRel CSet OptionR.
 Require Import Val Var Env IL Annotation Infra.Lattice DecSolve.
 Require Import Analysis.Analysis AnalysisForwardSSA ValueOpts.ConstantPropagation.
 
-Require Import CMap WithTop.
+Require Import CMap WithTop DomainSSA.
 
 Set Implicit Arguments.
 
@@ -28,23 +28,7 @@ Smpl Add 100 match goal with
              end : inv_trivial.
 
 Require Import MapNotations ListUpdateAt Subterm.
-
-Definition domupd (d:Dom) x (o:aval) : Dom :=
-  match o with
-  | Some xv => (d [- x <- xv -])
-  | None => remove x d
-  end.
-
-Fixpoint domupd_list (m:Dom) (A:list var) (B:list aval) :=
-  match A, B with
-  | x::A, y::B =>
-    domupd (domupd_list m A B) x (join (find x m) y)
-  | _, _ => m
-  end.
-
-Definition domenv (d:Dom) (x:var) : aval :=
-  find x d.
-
+(*
 Instance eq_Refl
   : Reflexive (fun p p' : Dom * params => fst p ≣ fst p' /\ snd p = snd p').
 Proof.
@@ -83,45 +67,6 @@ Proof.
 Qed.
 
 Require Import Terminating OptionR.
-
-Lemma leMap_op_eval e a b
-  : leMap a b
-    -> poLe (op_eval (domenv a) e) (op_eval (domenv b) e).
-Proof.
-  general induction e; simpl; eauto using @fstNoneOrR, @withTop_le.
-  - reflexivity.
-  - unfold domenv.
-    specialize (H n).
-    destruct (find n a); eauto using fstNoneOrR.
-  - specialize (IHe _ _ H); repeat cases; eauto using fstNoneOrR, @withTop_le.
-    reflexivity.
-  - specialize (IHe1 _ _ H).
-    specialize (IHe2 _ _ H).
-    inv IHe1; inv IHe2; repeat cases;
-      simpl in *; clear_trivial_eqs;
-        eauto using fstNoneOrR, withTop_le.
-    + econstructor; econstructor. congruence.
-Qed.
-
-Lemma eqMap_op_eval e a b
-  : eqMap a b
-    -> poEq (op_eval (domenv a) e) (op_eval (domenv b) e).
-Proof.
-  general induction e; simpl; eauto using @fstNoneOrR, @withTop_eq, @option_R.
-  - reflexivity.
-  - unfold domenv.
-    specialize (H n).
-    destruct (find n a); eauto using fstNoneOrR.
-  - specialize (IHe _ _ H); repeat cases; eauto using fstNoneOrR, @withTop_eq, @option_R.
-    reflexivity.
-  - specialize (IHe1 _ _ H).
-    specialize (IHe2 _ _ H).
-    inv IHe1; inv IHe2; repeat cases;
-      simpl in *; clear_trivial_eqs;
-        eauto using fstNoneOrR, withTop_eq, option_R.
-    + econstructor; econstructor. congruence.
-Qed.
-
 
 Lemma poLe_option_None X `{PartialOrder X} (x:option X)
   :  ⎣⎦ ⊑ x.
@@ -206,6 +151,49 @@ Proof.
     eapply IHZ.
 Qed.
 
+ *)
+
+Lemma leMap_op_eval e a b
+  : poLe a b
+    -> poLe (op_eval (domenv a) e) (op_eval (domenv b) e).
+Proof.
+  general induction e; simpl; eauto using @fstNoneOrR, @withTop_le.
+  - reflexivity.
+  - unfold domenv.
+    specialize (H n).
+    destruct (find n a); eauto using fstNoneOrR.
+  - specialize (IHe _ _ H); repeat cases; eauto using fstNoneOrR, @withTop_le.
+    reflexivity.
+  - specialize (IHe1 _ _ H).
+    specialize (IHe2 _ _ H).
+    inv IHe1; inv IHe2; repeat cases;
+      simpl in *; clear_trivial_eqs;
+        eauto using fstNoneOrR, withTop_le.
+    + econstructor; econstructor. congruence.
+Qed.
+
+Hint Resolve leMap_op_eval.
+
+Lemma eqMap_op_eval e a b
+  : poEq a b
+    -> poEq (op_eval (domenv a) e) (op_eval (domenv b) e).
+Proof.
+  general induction e; simpl; eauto using @fstNoneOrR, @withTop_eq, @option_R.
+  - reflexivity.
+  - unfold domenv.
+    specialize (H n).
+    destruct (find n a); eauto using fstNoneOrR.
+  - specialize (IHe _ _ H); repeat cases; eauto using fstNoneOrR, @withTop_eq, @option_R.
+    reflexivity.
+  - specialize (IHe1 _ _ H).
+    specialize (IHe2 _ _ H).
+    inv IHe1; inv IHe2; repeat cases;
+      simpl in *; clear_trivial_eqs;
+        eauto using fstNoneOrR, withTop_eq, option_R.
+    + econstructor; econstructor. congruence.
+Qed.
+
+Hint Resolve leMap_op_eval eqMap_op_eval.
 
 Definition constant_propagation_transform sT ZL st (ST:subTerm st sT)
            (a:Dom) (b:bool)
@@ -224,7 +212,7 @@ Definition constant_propagation_transform sT ZL st (ST:subTerm st sT)
     (* we assume renamed apart here, so it's ok to leave definitions
        in d[X <-- Yc] that are /not/ defined at the point where f is defined *)
     if b then
-      domupd_list d Z Yc
+      domjoin_list d Z Yc
     else
       d
   | stmtReturn e as st, d =>
@@ -233,6 +221,39 @@ Definition constant_propagation_transform sT ZL st (ST:subTerm st sT)
     (* we assume renamed apart here, and dont zero Z *)
     d
   end.
+
+Arguments poLe : simpl never.
+Arguments poEq : simpl never.
+
+Lemma poLe_map D `{PartialOrder D} D' `{PartialOrder D'} (f g:D -> D') (L L':list D)
+      (LEf:forall a b, poLe a b -> poLe (f a) (g b))
+      (LE: poLe L L')
+  : poLe (f ⊝ L) (g ⊝ L').
+Proof.
+  general induction LE; simpl; eauto.
+Qed.
+
+Lemma poLe_map_nd D D' `{PartialOrder D'} (f g:D -> D') (L L':list D)
+      (LEf:forall a, poLe (f a) (g a))
+  : poLe (f ⊝ L) (g ⊝ L).
+Proof.
+  general induction L; simpl; eauto.
+Qed.
+
+Lemma poEq_map D `{PartialOrder D} D' `{PartialOrder D'} (f g:D -> D') (L L':list D)
+      (LEf:forall a b, poEq a b -> poEq (f a) (g b))
+      (LE: poEq L L')
+  : poLe (f ⊝ L) (g ⊝ L').
+Proof.
+  general induction LE; simpl; eauto.
+Qed.
+
+Lemma poEq_map_nd D D' `{PartialOrder D'} (f g:D -> D') (L L':list D)
+      (LEf:forall a, poEq (f a) (g a))
+  : poEq (f ⊝ L) (g ⊝ L).
+Proof.
+  general induction L; simpl; eauto.
+Qed.
 
 Lemma transf_mon
   : (forall (sT s : stmt) (ST : subTerm s sT) (ZL : 〔params〕) (a b : Dom),
@@ -244,40 +265,19 @@ Proof.
   general induction s; simpl in *; eauto.
   - destruct e; eauto.
     + eapply domupd_le; eauto.
-      eapply (leMap_op_eval e); eauto.
     + hnf; intros. mlud; eauto.
   - destruct (get_dec ZL l); dcr.
     + erewrite get_nth; eauto; simpl.
       repeat cases; isabsurd; eauto;
-        try (eapply domupd_list_le; eauto).
-      etransitivity; eauto.
-      eapply domupd_list_exp.
+        try (eapply domjoin_list_le; eauto).
+      * eapply poLe_map_nd; eauto.
+      * rewrite H. eapply domjoin_list_exp.
     + rewrite not_get_nth_default; eauto.
       simpl; repeat cases; eauto.
 Qed.
 
 
 Definition DDom (sT:stmt) := { m : Map [var, withTop val] | domain m ⊆ occurVars sT}.
-
-Lemma domain_domupd_incl m x v
-  : domain (domupd m x v) ⊆ {x; domain m}.
-Proof.
-  unfold domupd; cases.
-  - rewrite domain_add. reflexivity.
-  - rewrite domain_remove. cset_tac.
-Qed.
-
-Lemma domain_domupd_list_incl m x v
-  : domain (domupd_list m x v) ⊆ of_list x ∪ domain m.
-Proof.
-  general induction x; destruct v; simpl.
-  - cset_tac.
-  - cset_tac.
-  - cset_tac.
-  - rewrite domain_domupd_incl.
-    rewrite IHx; eauto. cset_tac.
-Qed.
-
 
 Lemma cp_trans_domain  sT (ZL:list params) st (ST:subTerm st sT)
        (ZLIncl: list_union (of_list ⊝ ZL) ⊆ occurVars sT) (a:DDom sT) b
@@ -290,7 +290,7 @@ Proof.
     rewrite domain_add. cset_tac.
   - destruct (get_dec ZL l); dcr.
     + erewrite get_nth; eauto; cases; eauto.
-      rewrite domain_domupd_list_incl.
+      rewrite domain_domjoin_list_incl.
       eapply union_incl_split; eauto.
       rewrite <- ZLIncl.
       eapply incl_list_union; eauto using map_get_1.
@@ -317,6 +317,7 @@ Proof.
   intros. destruct a as [a aBound], b as [b bBound]; simpl in H.
   pose proof (@transf_mon sT s ST ZL a b H) as LE.
   destruct s; clear_trivial_eqs; simpl in *; eauto.
+  eapply LE; eauto.
 Qed.
 
 
@@ -329,88 +330,14 @@ Proof.
   intros. unfold cp_trans_dep; cases; simpl; eauto.
   - cases; eauto.
     + eapply domupd_eq; eauto.
-      eapply eqMap_op_eval; eauto.
-    + hnf; intros. mlud; eauto.
+    + hnf; intros. simpl. mlud; eauto.
   - repeat cases; eauto.
+    eapply poEq_vdom_struct.
     destruct (get_dec ZL l); dcr.
     + erewrite get_nth; eauto.
-      eapply domupd_list_eq; eauto.
+      eapply domjoin_list_eq; eauto.
+      eapply poEq_map_nd; eauto.
     + rewrite not_get_nth_default; eauto; simpl; cases; eauto.
-Qed.
-
-Lemma domain_join_sig X `{OrderedType X} Y `{JoinSemiLattice Y}  U
-  (x y : {m : Map [X, Y] | domain m [<=] U})
-  : domain (proj1_sig x ⊔ proj1_sig y) [<=] U.
-Proof.
-  destruct x,y; simpl.
-  unfold joinMap. rewrite domain_join. cset_tac.
-Qed.
-
-Definition joinsig X `{OrderedType X} Y `{JoinSemiLattice Y}  U
-           (x y : {m : Map [X, Y] | domain m ⊆ U}) :=
-  exist (fun m => domain m ⊆ U) (join (proj1_sig x) (proj1_sig y)) (domain_join_sig x y).
-
-Definition joinsig_idem X `{OrderedType X} Y `{JoinSemiLattice Y}  U
-  : forall a : {m : Map [X, Y] | domain m [<=] U}, joinsig a a ≣ a.
-Proof.
-  - hnf; intros [a ?]. simpl. eapply joinDom_idem.
-Qed.
-
-Definition joinsig_sym X `{OrderedType X} Y `{JoinSemiLattice Y}  U
-  : forall a b : {m : Map [X, Y] | domain m [<=] U}, joinsig a b ≣ joinsig b a.
-Proof.
-  - hnf; intros [a ?] [b ?]. eapply joinDom_sym.
-Qed.
-
-Definition joinsig_assoc X `{OrderedType X} Y `{JoinSemiLattice Y}  U
-  : forall a b c : {m : Map [X, Y] | domain m [<=] U}, joinsig (joinsig a b) c ≣ joinsig a (joinsig b c).
-Proof.
-  hnf; intros [a ?] [b ?] [c ?]. eapply joinDom_assoc.
-Qed.
-
-Definition joinsig_exp X `{OrderedType X} Y `{JoinSemiLattice Y}  U
-  : forall a b : {m : Map [X, Y] | domain m [<=] U}, a ⊑ joinsig a b.
-Proof.
-  hnf; intros [a ?] [b ?]; simpl. eapply joinDom_exp.
-Qed.
-
-
-Instance map_sig_semilattice_bound X `{OrderedType X} Y `{JoinSemiLattice Y}  U
-  : JoinSemiLattice ({ m : Map [X, Y] | domain m ⊆ U}) := {
-  join x y := joinsig x y
-}.
-Proof.
-  - eapply joinsig_idem.
-  - eapply joinsig_sym.
-  - eapply joinsig_assoc.
-  - eapply joinsig_exp.
-  - simpl. unfold Proper, respectful; intros. destruct x,y,x0,y0; simpl in * |- *.
-    rewrite H2, H3. reflexivity.
-  - simpl. unfold Proper, respectful; intros. destruct x,y,x0,y0; simpl in * |- *.
-    rewrite H3, H2. reflexivity.
-Defined.
-
-Instance map_sig_lower_bounded X `{OrderedType X} Y `{JoinSemiLattice Y} U
-  : LowerBounded { m : Map [X, Y] | domain m ⊆ U} :=
-  {
-    bottom := exist _ (empty _) (incl_empty _ _)
-  }.
-Proof.
-  intros [a b]; simpl.
-  eapply empty_bottom; eauto.
-Defined.
-
-Instance
-  : Terminating (withTop val) poLt.
-Proof.
-  hnf; intros.
-  destruct x.
-  - econstructor; intros. inv H. inv H0. inv H. exfalso; eauto.
-  - econstructor; intros. inv H. inv H0.
-    + eapply int_eq_eq in H3. subst.
-      exfalso. eapply H1. eauto.
-    + econstructor; intros.
-      inv H2. inv H3. inv H2. exfalso; eauto.
 Qed.
 
 Definition cp_trans_reach (sT : stmt) (e : op)
@@ -422,6 +349,11 @@ Definition cp_trans_reach (sT : stmt) (e : op)
      else if [op_eval (domenv (proj1_sig d)) e = Some (wTA val_true)] then
             false else b).
 
+Smpl Add match goal with
+         | [ H : poLe _ None |- _ ] => invc H
+         | [ H : ⎣ ?x ⎦ <> ⎣ ?x ⎦ |- _ ] => exfalso; apply H; reflexivity
+         end : inv_trivial.
+
 Lemma cp_trans_reach_mon
   : forall (sT : stmt) (e : op) (s : stmt),
     subTerm s sT ->
@@ -430,17 +362,14 @@ Lemma cp_trans_reach_mon
       forall b b' : bool,
         b ⊑ b' -> cp_trans_reach e FVIncl a b ⊑ cp_trans_reach e FVIncl a' b'.
 Proof.
-  intros. exploit (leMap_op_eval e); eauto. eapply H0.
+  intros. pose proof (leMap_op_eval e H0); eauto.
   unfold cp_trans_reach.
   set (X:=op_eval (domenv (proj1_sig a)) e) in *.
   set (Y:=op_eval (domenv (proj1_sig a')) e) in *. clearbody X Y.
-  repeat cases; split; simpl fst; simpl snd; eauto.
+  unfold val in *.
+  repeat cases; split; simpl fst; simpl snd; eauto; clear_trivial_eqs.
   inv H2; clear_trivial_eqs.
   inv H2; clear_trivial_eqs.
-  inv H2; clear_trivial_eqs.
-  exfalso; eauto.
-  inv H2; clear_trivial_eqs.
-  exfalso; eauto.
 Qed.
 
 Lemma cp_trans_reach_ext
@@ -459,7 +388,27 @@ Proof.
   inv H2; clear_trivial_eqs; exfalso; eauto.
 Qed.
 
+
+Definition cp_reach (U : ⦃nat⦄) (b:bool) (d: VDom U (withTop val)) (e:op) : bool * bool :=
+  (true, true).
+
+Lemma cp_reach_mon (U : ⦃nat⦄) (e : op) (a a' : VDom U (withTop val))
+  : a ⊑ a' -> forall b b' : bool, b ⊑ b' -> cp_reach b a e ⊑ cp_reach b' a' e.
+Proof.
+  intros. reflexivity.
+Qed.
+
+Definition cp_trans (U : ⦃nat⦄) (b:bool) (d: VDom U (withTop val)) (e:exp) : ؟ (withTop val) :=
+  match e with
+  | Operation e => op_eval (domenv (proj1_sig d)) e
+  | _ => Some Top
+  end.
+
+Lemma cp_trans_mon (U : ⦃nat⦄) (e : exp) (a a' : VDom U (withTop val))
+  : a ⊑ a' -> forall b b' : bool, b ⊑ b' -> @cp_trans U b a e ⊑ @cp_trans U b' a' e.
+Proof.
+  intros. destruct e; simpl; eauto.
+Qed.
+
 Definition constant_propagation_analysis :=
-  makeForwardAnalysis DDom _ _ cp_trans_dep cp_trans_reach
-                      transf_mon_dep cp_trans_reach_mon
-                      (fun s => (@terminating_Dom var _ _ _ (occurVars s) _)).
+  makeForwardAnalysis _ _ _ cp_trans cp_reach cp_trans_mon cp_reach_mon.
